compiler/backend/proofs/bvl_to_bviProofScript.sml
@@ -627,63 +627,95 @@ val evaluate_CopyGlobals_code = Q.prove(
   |> Q.GEN`ls`;
 val _ = print "Proved evaluate_CopyGlobals_code\n"
 
-val evaluate_AllocGlobal_code = Q.prove(
-  `s.global = SOME p ∧
+Theorem evaluate_AllocGlobal_code[local]:
    FLOOKUP s.refs p = SOME (ValueArray (Number(&(SUC n))::ls)) ∧ n ≤ LENGTH ls ∧
+   s.global = SOME p ∧
    lookup CopyGlobals_location s.code = SOME (3,SND CopyGlobals_code)
    ⇒
-   ∃p1 c.
+   ∃p1 c extra.
      (p1 ≠ p ⇒ p1 ∉ FDOM s.refs) ∧
-     evaluate ([SND AllocGlobal_code],[],inc_clock c s) =
+     n+k+1 ≤ LENGTH ls + extra ∧
+     evaluate ([SND AllocGlobal_code],[Number (& k)],inc_clock c s) =
        (Rval [Unit],
         s with <| global := SOME p1; refs := s.refs
-          |+ (p, ValueArray ((Number(&(SUC(n+1))))::ls))
-          |+ (p1, ValueArray ((Number(&(SUC(n+1))))::
-                              if n < LENGTH ls then ls
-                              else ls ++ (REPLICATE (SUC(LENGTH ls)) (Number 0))))|>)`,
-  strip_tac >>
-  simp[AllocGlobal_code_def,iEval_def,iEvalOp_def,do_app_aux_def,backend_commonTheory.small_enough_int_def,
-       Once inc_clock_def,bEvalOp_def,bvl_to_bvi_id,bvl_to_bvi_with_refs,FLOOKUP_UPDATE,
-       find_code_def] >>
-  IF_CASES_TAC >> simp[] >- (
-    Q.LIST_EXISTS_TAC[`p`,`0`] >>
-    simp[state_component_equality] >>
-    EVAL_TAC >>
-    simp[fmap_eq_flookup,FLOOKUP_UPDATE] >>
-    srw_tac[][] >> simp[] >> intLib.COOPER_TAC) >>
-  `(λptr. ptr ≠ p ∧ ptr ∉ FDOM s.refs) = (λptr. ptr ∉ FDOM s.refs)` by (
-    simp[FUN_EQ_THM] >> full_simp_tac(srw_ss())[FLOOKUP_DEF] >> metis_tac[]) >> simp[] >>
-  qpat_abbrev_tac`p1 = LEAST ptr. ptr ∉ FDOM s.refs` >>
-  qexists_tac`p1` >>
-  `p1 ∉ FDOM s.refs` by (
-    rpt strip_tac >> full_simp_tac(srw_ss())[FLOOKUP_DEF] >>
-    metis_tac[LEAST_NOTIN_FDOM] ) >>
-  simp[LUPDATE_def] >>
-  qpat_abbrev_tac`l1 = REPLICATE _ _` >>
-  qpat_abbrev_tac`rf = s.refs |+ _ |+ _` >>
-  qspecl_then[`Number(1+ &SUC n)::ls`,`n`,`l1`,`s with <| global := SOME p1; refs := rf|>`]mp_tac evaluate_CopyGlobals_code >>
-  impl_tac >- (
-    simp[Abbr`rf`,FLOOKUP_UPDATE] >>
-    IF_CASES_TAC >> simp[] >- (
-      full_simp_tac(srw_ss())[FLOOKUP_DEF] >> metis_tac[LEAST_NOTIN_FDOM] ) >>
-    simp[Abbr`l1`,LENGTH_REPLICATE] \\ intLib.COOPER_TAC ) >>
-  strip_tac >>
-  qexists_tac`c+1` >>
-  simp[] >>
-  qpat_abbrev_tac`ss = dec_clock 1 Z` >>
-  `ss = inc_clock c (s with <| global := SOME p1; refs := rf|>)` by (
-    simp[Abbr`ss`] >> EVAL_TAC >>
-    simp[state_component_equality] ) >>
-  simp[Abbr`ss`] >>
-  `&SUC n - 1 = &n:int` by (Cases_on`n`>>full_simp_tac(srw_ss())[]>>simp[ADD1]>>intLib.COOPER_TAC) >> full_simp_tac(srw_ss())[] >>
-  simp[Abbr`rf`,fmap_eq_flookup,FLOOKUP_UPDATE,state_component_equality] >>
-  srw_tac[][] >> simp[] >> TRY(intLib.COOPER_TAC) >>
-  `n = LENGTH ls`by decide_tac >>
-  `2 * (LENGTH ls + 1) = LENGTH ls + LENGTH ls + 2` by DECIDE_TAC >>
-  simp[Abbr`l1`,DROP_REPLICATE,ADD1]
-  \\ rewrite_tac[GSYM REPLICATE]
-  \\ AP_THM_TAC \\ AP_TERM_TAC
-  \\ intLib.COOPER_TAC);
+          |+ (p, ValueArray ((Number(&(SUC(n+k))))::ls))
+          |+ (p1, ValueArray ((Number(&(SUC(n+k))))::
+                              ls ++ (REPLICATE extra (Number 0))))|>)
+Proof
+  strip_tac
+  \\ simp [AllocGlobal_code_def]
+  \\ simp [Once iEval_def,iEvalOp_def]
+  \\ simp [Once iEval_def,iEvalOp_def,inc_clock_def,do_app_aux_def]
+  \\ simp [Once iEval_def,iEvalOp_def,inc_clock_def,do_app_aux_def]
+  \\ simp [Once iEval_def,iEvalOp_def,inc_clock_def,do_app_aux_def]
+  \\ simp [Once iEval_def,iEvalOp_def,inc_clock_def,do_app_aux_def]
+  \\ simp [Once iEval_def,iEvalOp_def,inc_clock_def,do_app_aux_def]
+  \\ simp [Once iEval_def,iEvalOp_def,inc_clock_def,do_app_aux_def]
+  \\ simp [Once iEval_def,iEvalOp_def,inc_clock_def,do_app_aux_def]
+  \\ simp [Once iEval_def,iEvalOp_def,inc_clock_def,do_app_aux_def]
+  \\ simp [EVAL “small_enough_int 0”]
+  \\ simp [Once iEval_def,iEvalOp_def,inc_clock_def,do_app_aux_def,bvlSemTheory.do_app_def]
+  \\ rename [‘evaluate
+                ([Op Add [Var 0; Var 2]],
+                 [Number (&SUC n); RefPtr p; Number (&k)],_)’]
+  \\ simp [Once iEval_def]
+  \\ simp [Once iEval_def]
+  \\ simp [Once iEval_def]
+  \\ simp [Once iEval_def]
+  \\ simp [iEvalOp_def,inc_clock_def,do_app_aux_def,bvlSemTheory.do_app_def]
+  \\ simp [Once iEval_def]
+  \\ simp [Once iEval_def]
+  \\ simp [Once iEval_def]
+  \\ simp [iEvalOp_def,inc_clock_def,do_app_aux_def,bvlSemTheory.do_app_def]
+  \\ simp [bvl_to_bvi_def,bvi_to_bvl_def]
+  \\ ntac 8 $ simp [Once iEval_def]
+  \\ simp [iEvalOp_def,do_app_aux_def,bvlSemTheory.do_app_def]
+  \\ simp [EVAL “small_enough_int 0”]
+  \\ ntac 5 $ simp [Once iEval_def]
+  \\ simp [iEvalOp_def,do_app_aux_def,bvlSemTheory.do_app_def,integerTheory.INT_ADD]
+  \\ fs [ADD1] \\ CASE_TAC
+  >-
+   (gvs [bvl_to_bvi_def,bvi_to_bvl_def,iEval_def,state_component_equality]
+    \\ qexists_tac ‘0’ \\ gvs [LUPDATE_def])
+  \\ gvs [bvl_to_bvi_def,bvi_to_bvl_def]
+  \\ ntac 5 $ simp [Once iEval_def]
+  \\ simp [iEvalOp_def,do_app_aux_def,bvlSemTheory.do_app_def]
+  \\ simp [EVAL “small_enough_int 0”]
+  \\ ntac 5 $ simp [Once iEval_def]
+  \\ simp [iEvalOp_def,do_app_aux_def,bvlSemTheory.do_app_def,integerTheory.INT_ADD]
+  \\ gvs [bvl_to_bvi_def,bvi_to_bvl_def]
+  \\ ntac 2 $ simp [Once iEval_def]
+  \\ simp [iEvalOp_def,do_app_aux_def,bvlSemTheory.do_app_def,integerTheory.INT_ADD]
+  \\ ntac 10 $ simp [Once iEval_def]
+  \\ simp [iEvalOp_def,do_app_aux_def,bvlSemTheory.do_app_def]
+  \\ simp [EVAL “small_enough_int 0”,EVAL “small_enough_int 1”]
+  \\ gvs [bvl_to_bvi_def,bvi_to_bvl_def,find_code_def,dec_clock_def]
+  \\ qabbrev_tac ‘new_p = LEAST ptr. ptr ≠ p ∧ ptr ∉ FDOM s.refs’
+  \\ qexists_tac ‘new_p’ \\ fs []
+  \\ Q.REFINE_EXISTS_TAC ‘ccc+1’ \\ fs []
+  \\ gvs [AllCaseEqs()]
+  \\ qpat_abbrev_tac ‘new_refs = _ |+ _ |+ _’
+  \\ simp [GSYM integerTheory.INT_ADD,int_arithTheory.elim_minus_ones]
+  \\ qabbrev_tac ‘s1 = s with <| refs := new_refs ; global := SOME new_p; ffi := s.ffi |>’
+  \\ ‘lookup CopyGlobals_location s1.code = SOME (3,SND CopyGlobals_code)’
+        by fs [Abbr‘s1’]
+  \\ drule (GEN_ALL evaluate_CopyGlobals_code)
+  \\ disch_then $ qspecl_then [‘new_p’,‘p’] mp_tac
+  \\ ‘p ≠ new_p ∧ new_p ∉ FDOM s.refs’ by
+    (`∃x. (λptr. ptr NOTIN FDOM (s.refs |+ (p,ARB))) x` by
+          (SIMP_TAC std_ss [] \\ METIS_TAC [NUM_NOT_IN_FDOM])
+     \\ drule whileTheory.LEAST_INTRO \\ fs [])
+  \\ fs []
+  \\ simp [Abbr‘s1’,FLOOKUP_UPDATE,Abbr‘new_refs’,inc_clock_def]
+  \\ disch_then $ qspec_then ‘LENGTH ls’ mp_tac
+  \\ impl_tac >- gvs []
+  \\ strip_tac \\ gvs [LUPDATE_def]
+  \\ qexists_tac ‘c’ \\ fs []
+  \\ simp [state_component_equality]
+  \\ qmatch_goalsub_abbrev_tac ‘REPLICATE kk’
+  \\ qexists_tac ‘kk’ \\ fs [Abbr‘kk’]
+  \\ simp [integerTheory.INT_ADD]
+QED
 
 Theorem evaluate_ListLength_code:
    !lv vs n.
@@ -2909,65 +2941,63 @@ Proof
          srw_tac[][] >- ( full_simp_tac(srw_ss())[FLOOKUP_DEF] >> srw_tac[][] >> METIS_TAC[] ) >>
          qexists_tac`z` >> simp[ADD1,LUPDATE_MAP] >>
          simp[libTheory.the_def])
-    \\ Cases_on`op = AllocGlobal` \\ full_simp_tac(srw_ss())[] THEN1 (
-         note_tac "Op: AllocGlobal" >> simp[compile_op_def] >>
-         full_simp_tac(srw_ss())[bEvalOp_def] >>
-         Cases_on`REVERSE a`>>full_simp_tac(srw_ss())[]>>srw_tac[][]>>
-         imp_res_tac evaluate_IMP_LENGTH >>
-         full_simp_tac(srw_ss())[LENGTH_NIL] >> srw_tac[][] >>
-         srw_tac[][iEval_def] >>
-         simp[Once inc_clock_def] >>
-         simp[find_code_def] >>
-         `lookup AllocGlobal_location t1.code = SOME(0,SND AllocGlobal_code)` by (
-           full_simp_tac(srw_ss())[state_rel_def] >> simp[AllocGlobal_code_def] ) >>
-         simp[] >>
-         let
-           val th = (Q.ISPEC`inc_clock c (t1:('c,'ffi) bviSem$state)`(Q.GEN`s`evaluate_AllocGlobal_code))
-         in
-         Q.SUBGOAL_THEN `∃p n ls. ^(fst(dest_imp(concl th)))` assume_tac
-         THEN1 (
-           full_simp_tac(srw_ss())[state_rel_def,REPLICATE_NIL] >>
-           simp[Once inc_clock_def] >>
-           simp[CopyGlobals_code_def] >>
-           Cases_on`t1.global`>>full_simp_tac(srw_ss())[])
-         end >>
-         rpt(pop_assum CHOOSE_TAC) >>
-         first_assum(mp_tac o MATCH_MP evaluate_AllocGlobal_code) >>
-         disch_then(qx_choosel_then[`p1`,`ck`]strip_assume_tac) >>
-         CONV_TAC(RESORT_EXISTS_CONV(List.rev)) >>
-         Q.LIST_EXISTS_TAC[`c+ck+1`,`b2`] >>
-         simp[Once inc_clock_def] >>
-         `dec_clock 1 (inc_clock (c + (ck+1)) t1) =
-          inc_clock ck (inc_clock c t1)` by (
-           EVAL_TAC >> simp[state_component_equality] ) >>
-         simp[] >>
-         ntac 2 (pop_assum kall_tac) >>
-         full_simp_tac(srw_ss())[iEval_def] >> var_eq_tac >>
-         full_simp_tac(srw_ss())[state_rel_def,LENGTH_REPLICATE,FLOOKUP_UPDATE] >>
+    \\ Cases_on`op = AllocGlobal` \\ full_simp_tac(srw_ss())[] THEN1
+        (note_tac "Op: AllocGlobal" \\ simp[compile_op_def]
+         \\ gvs [bvlSemTheory.do_app_def,AllCaseEqs()]
+         \\ rename [‘~(ii < 0:int)’]
+         \\ ‘∃k. ii = & k’ by (Cases_on ‘ii’ \\ gvs [])
+         \\ drule_then assume_tac bvlPropsTheory.evaluate_IMP_LENGTH
+         \\ gvs [LENGTH_EQ_NUM_compute]
+         \\ drule_then assume_tac compile_exps_LENGTH
+         \\ gvs [LENGTH_EQ_NUM_compute,adjust_bv_def]
+         \\ gvs [iEvalOp_def,iEval_def]
+         \\ `lookup AllocGlobal_location t2.code = SOME(1,SND AllocGlobal_code)` by
+           (fs [state_rel_def] \\ simp[AllocGlobal_code_def])
+         \\ simp [find_code_def]
+         \\ qpat_x_assum ‘state_rel b2 s5 t2’ mp_tac
+         \\ simp [Once state_rel_def]
+         \\ strip_tac
+         \\ drule evaluate_global_mono
+         \\ simp [Once inc_clock_def] \\ strip_tac
+         \\ Cases_on ‘t2.global’ \\ fs []
+         \\ drule evaluate_AllocGlobal_code
+         \\ simp []
+         \\ impl_tac
+         >- EVAL_TAC
+         \\ strip_tac
+         \\ qpat_x_assum ‘_ = (Rval [Number (&k)],t2)’ assume_tac
+         \\ drule evaluate_add_clock \\ fs []
+         \\ disch_then $ qspec_then ‘c'+1’ assume_tac
+         \\ fs [inc_clock_def] \\ full_simp_tac std_ss [ADD_ASSOC]
+         \\ simp [AllCaseEqs(),PULL_EXISTS]
+         \\ ‘c + c' + t1.clock + 1 = (c + c' + 1) + t1.clock’ by fs []
+         \\ full_simp_tac std_ss []
+         \\ first_assum $ irule_at $ Pos hd
+         \\ simp [dec_clock_def]
+         \\ first_assum $ irule_at $ Pos $ el 2
+         \\ conj_tac >- EVAL_TAC
+         \\ simp [state_rel_def,FLOOKUP_UPDATE]
+         \\ full_simp_tac(srw_ss())[iEval_def] >> rpt var_eq_tac >>
+         full_simp_tac(srw_ss())[LENGTH_REPLICATE,FLOOKUP_UPDATE] >>
          conj_tac >- full_simp_tac(srw_ss())[INJ_DEF] >>
          conj_tac >- (
            gen_tac >>
-           Cases_on`FLOOKUP s5.refs k`>>simp[]>>
-           `p ≠ b2 k` by ( full_simp_tac(srw_ss())[FLOOKUP_DEF] >> METIS_TAC[]) >>
-           `p1 ≠ b2 k` by (
+           Cases_on`FLOOKUP s5.refs k'`>>simp[]>>
+           `x ≠ b2 k'` by (
+             full_simp_tac(srw_ss())[INJ_DEF,FLOOKUP_DEF] >>
+             METIS_TAC[] ) >>
+           `p1 ≠ b2 k'` by (
              full_simp_tac(srw_ss())[INJ_DEF,FLOOKUP_DEF] >>
              METIS_TAC[] ) >>
            simp[] >>
-           rpt(first_x_assum(qspec_then`k`mp_tac)) >>
-           simp[] ) >>
+           rpt(first_x_assum(qspec_then`k'`mp_tac)) >>
+           simp[])  >>
          conj_tac >- (
            full_simp_tac(srw_ss())[FLOOKUP_DEF] >> metis_tac[INJ_DEF]) >>
-         IF_CASES_TAC >- (
-           qexists_tac`z'`>>simp[libTheory.the_def]>>
-           simp[LIST_EQ_REWRITE,LENGTH_REPLICATE,EL_REPLICATE] >>
-           Cases >> simp[EL_REPLICATE] ) >>
-         qexists_tac`z' * 2`>>simp[libTheory.the_def] >>
-         qmatch_abbrev_tac`REPLICATE a x ++ [x] ++ REPLICATE b x = _` >>
-         `REPLICATE a x ++ [x] ++ REPLICATE b x = REPLICATE (a + SUC b) x`
-         by simp[GSYM REPLICATE_APPEND] >>
-         `a + SUC b = SUC (a + b)` by simp[] >>
-         rw[] >>
-         simp[LIST_EQ_REWRITE,Abbr`a`,Abbr`b`,LENGTH_REPLICATE,EL_REPLICATE])
+         rewrite_tac [REPLICATE_APPEND,libTheory.the_def] >>
+         irule_at Any (METIS_PROVE [] “k = n ⇒ REPLICATE k x = REPLICATE n x”) >>
+         fs [ADD1] >>
+         qexists_tac ‘extra+z’ >> fs [])
     \\ Cases_on`∃part. op = EqualConst part` \\ fs[] >- (
       note_tac "Op: EqualConst" \\ gvs[compile_op_def,bEvalOp_def]
       \\ Cases_on`REVERSE a` \\ fs[] \\ rw[]
@@ -4080,25 +4110,29 @@ Proof
   \\ fs [FILTER_APPEND] \\ EVAL_TAC
 QED
 
-val ODD_lemma = prove(
-  ``ODD (2 * n + k) = ODD k``,
-  fs [ODD_ADD] \\ simp [ODD_EVEN,EVEN_DOUBLE]);
+Triviality ODD_lemma:
+  ODD (2 * n + k) = ODD k
+Proof
+  fs [ODD_ADD] \\ simp [ODD_EVEN,EVEN_DOUBLE]
+QED
 
-val full_cc_def = Define `
+Definition full_cc_def:
   full_cc c cc =
     let limit = c.inline_size_limit in
     let split = c.split_main_at_seq in
     let cut = c.exp_cut in
       state_cc (compile_inc limit split cut) (state_cc compile_inc
-        (state_cc bvi_tailrec$compile_prog cc))`
+        (state_cc bvi_tailrec$compile_prog cc))
+End
 
-val full_co_def = Define `
+Definition full_co_def:
   full_co c co =
     let limit = c.inline_size_limit in
     let split = c.split_main_at_seq in
     let cut = c.exp_cut in
       state_co bvi_tailrec$compile_prog (state_co compile_inc
-        (state_co (compile_inc limit split cut) co))`
+        (state_co (compile_inc limit split cut) co))
+End
 
 Theorem compile_prog_avoids_nss_2:
    compile_prog start f prog = (loc,code,new_state) /\
